src/proof/iam_model/aliases.v
@@ -1,12 +1,14 @@
 From New.proof Require Import prelude.
 From New.code Require Export iam_model.
-From iris.algebra Require Import gmap.
+From iris.algebra Require Import gmap gset.
 
-Definition identity_map : Type :=
-  gmap iammodel.IdentityID.t (gmap iammodel.PolicyID.t unit).
+Definition identity_set : Type := gset iammodel.IdentityID.t.
+
+Definition attachment : Type := (iammodel.IdentityID.t * iammodel.PolicyID.t)%type.
+
+Definition attachment_set : Type := gset attachment.
 
 Definition policy_map {ext : ffi_syntax} {go_gctx : GoGlobalContext} : Type :=
   gmap iammodel.PolicyID.t iammodel.IdentityPolicy.t.
 
-Definition policy_id_set : Type :=
-  gmap iammodel.PolicyID.t unit.
+Definition policy_id_set : Type := gset iammodel.PolicyID.t.
