src/proof/iam_model/inv.v
@@ -25,11 +25,11 @@ Local Set Default Proof Using "All".
 Instance policy_id_set_zero_val : ZeroVal policy_id_set :=
   {| zero_val := ∅ |}.
 
-Definition own_identities_auth γ (identities : identity_map) : iProp Σ :=
+Definition own_identities_auth γ (identities : identity_set) : iProp Σ :=
   own_identity_auth γ.(γ_identities) identities.
 
 Definition own_identity γ (identity : iammodel.IdentityID.t) : iProp Σ :=
-  ∃ policy_ids, own_identity_frag γ.(γ_identities) identity policy_ids.
+  own_identity_frag γ.(γ_identities) identity.
 
 Definition own_policies_auth γ (policies : policy_map) : iProp Σ :=
   own_policy_auth γ.(γ_policies) policies.
@@ -38,36 +38,41 @@ Definition own_policy γ (policy_id : iammodel.PolicyID.t) : iProp Σ :=
   ∃ policy, own_policy_frag γ.(γ_policies) policy_id policy.
 
 Definition own_resource_access_auth γ
-    (identities : identity_map) (policies : policy_map)
+    (identities : identity_set) (attachments : attachment_set) (policies : policy_map)
     (observed_resources : gset iammodel.ResourceName.t) : iProp Σ :=
   own_reversed_identity_policy_auth γ.(γ_resource_access)
-    identities policies observed_resources.
+    identities attachments policies observed_resources.
 
 Definition iam_inv γ l : iProp Σ :=
   ∃ (phys_identities_l : loc) (phys_policies_l : loc)
+    (phys_attachments_l : loc)
     (phys_used_policy_ids_l : loc)
-    (phys_identities : identity_map)
+    (phys_identities : identity_set)
+    (phys_attachments : attachment_set)
     (phys_policies : policy_map)
     (phys_used_policy_ids : policy_id_set)
     (observed_resources : gset iammodel.ResourceName.t),
     "Hstate_identities_addr" ∷ l.[(iammodel.State.t), "identities"] ↦ phys_identities_l ∗
     "Hstate_policies_addr" ∷ l.[(iammodel.State.t), "policies"] ↦ phys_policies_l ∗
+    "Hstate_attachments_addr" ∷ l.[(iammodel.State.t), "attachments"] ↦ phys_attachments_l ∗
     "Hstate_used_policy_ids_addr" ∷
       l.[(iammodel.State.t), "usedPolicyIds"] ↦ phys_used_policy_ids_l ∗
-    "Hown_phys_identities" ∷ phys_identities_l ↦$ phys_identities ∗
+    "Hown_phys_identities" ∷ phys_identities_l ↦$ gset_to_gmap tt phys_identities ∗
     "Hown_phys_policies" ∷ phys_policies_l ↦$ phys_policies ∗
-    "Hown_phys_used_policy_ids" ∷ phys_used_policy_ids_l ↦$ phys_used_policy_ids ∗
+    "Hown_phys_attachments" ∷ phys_attachments_l ↦$ gset_to_gmap tt phys_attachments ∗
+    "Hown_phys_used_policy_ids" ∷
+      phys_used_policy_ids_l ↦$ gset_to_gmap tt phys_used_policy_ids ∗
     "Hidentities" ∷ own_identities_auth γ phys_identities ∗
     "Hpolicies" ∷ own_policies_auth γ phys_policies ∗
     "Hresource_access" ∷
-      own_resource_access_auth γ phys_identities phys_policies observed_resources ∗
-    "%Hattached_policy_exists" ∷ ⌜ ∀ identity policy_ids policy_id,
-      phys_identities !! identity = Some policy_ids →
-      policy_ids !! policy_id = Some tt →
+      own_resource_access_auth γ phys_identities phys_attachments phys_policies observed_resources ∗
+    "%Hattachments_valid" ∷ ⌜ ∀ identity policy_id,
+      (identity, policy_id) ∈ phys_attachments →
+      identity ∈ phys_identities ∧
       ∃ policy, phys_policies !! policy_id = Some policy ⌝ ∗
     "%Hexisting_policy_used" ∷ ⌜ ∀ policy_id policy,
       phys_policies !! policy_id = Some policy →
-      phys_used_policy_ids !! policy_id = Some tt ⌝.
+      policy_id ∈ phys_used_policy_ids ⌝.
 
 Definition is_iam γ l : iProp Σ :=
   ∃ (mu_l : loc),
@@ -98,8 +103,8 @@ Global Instance own_policy_persistent γ policy_id :
   Persistent (own_policy γ policy_id).
 Proof. unfold own_policy. apply _. Qed.
 
-Global Instance own_resource_access_auth_timeless γ identities policies observed_resources :
-  Timeless (own_resource_access_auth γ identities policies observed_resources).
+Global Instance own_resource_access_auth_timeless γ identities attachments policies observed_resources :
+  Timeless (own_resource_access_auth γ identities attachments policies observed_resources).
 Proof. unfold own_resource_access_auth. apply _. Qed.
 
 End inv.
